Regex/Syntax/Translate.lean
@@ -155,9 +155,33 @@ private def hir_perl_unicode_class (cls : AstItems.ClassPerl) (flags : Flags)
   | .Space =>
     let range : Array ClassUnicodeRange ← range_of_property "White_Space"
     Except.ok (unicode_fold_and_negate range flags cls.negated)
+  | .VerticalSpace =>
+    let range1 : Array ClassUnicodeRange ← range_of_property "White_Space"
+    let range2 : Array ClassUnicodeRange :=
+      #[⟨⟨'\u0009', '\u0009'⟩, by simp_arith⟩, ⟨⟨'\u0020', '\u0020'⟩, by simp_arith⟩, ⟨⟨'\u00a0', '\u00a0'⟩, by simp_arith⟩]
+    let is1 : IntervalSet Char := IntervalSet.canonicalize range1
+    let is2 : IntervalSet Char := IntervalSet.canonicalize range2
+    let diff := IntervalSet.difference is1 is2
+    Except.ok (if cls.negated then ⟨IntervalSet.negate diff⟩ else ⟨diff⟩)
+  | .HorizontalSpace =>
+    let range1 : Array ClassUnicodeRange ← range_of_property "White_Space"
+    let range2 : Array ClassUnicodeRange := #[⟨⟨'\u000a', '\u000a'⟩, by simp_arith⟩]
+    let is1 : IntervalSet Char := IntervalSet.canonicalize range1
+    let is2 : IntervalSet Char := IntervalSet.canonicalize range2
+    let diff := IntervalSet.difference is1 is2
+    Except.ok (if cls.negated then ⟨IntervalSet.negate diff⟩ else ⟨diff⟩)
   | .Word =>
     let range : Array ClassUnicodeRange := ← range_of_property "Word"
     Except.ok (unicode_fold_and_negate range flags cls.negated)
+  | .Newline =>
+    if cls.negated then
+      let range1 : ClassUnicodeRange := ⟨⟨'\u0000', '\u0009'⟩, by simp_arith⟩
+      let range2 : ClassUnicodeRange := ⟨⟨'\u000B', ⟨0xD7FF, by simp_arith⟩⟩, by simp_arith⟩
+      let range3 : ClassUnicodeRange := ⟨⟨⟨0xE000, by simp_arith⟩, ⟨0x10FFFF, by simp_arith⟩⟩, by simp_arith⟩
+      Except.ok ⟨IntervalSet.canonicalize #[range1, range2, range3]⟩
+    else
+      let range1 : ClassUnicodeRange := ⟨⟨'\u000a', '\u000b'⟩, by simp_arith⟩
+      Except.ok ⟨IntervalSet.canonicalize #[range1]⟩
 
 private def hir_ascii_unicode_class (cls: AstItems.ClassAscii) (flags : Flags)
     : Except String ClassUnicode := do
@@ -216,6 +240,10 @@ private def hir_assertion (ast : AstItems.Assertion) (flags : Syntax.Flags) : Hi
       HirKind.Look (Look.WordStartHalfUnicode)
   | .WordBoundaryEndHalf =>
       HirKind.Look (Look.WordEndHalfUnicode)
+  | .PreviousMatch =>
+      HirKind.Look (Look.PreviousMatch)
+  | .ClearMatches =>
+      HirKind.Look (Look.ClearMatches)
 
   ⟨kind, Syntax.Hir.toProperties kind⟩
 
