testdata/pcre/readme.md
@@ -1,7 +1,7 @@
 # PCRE2 Testdata
 
 The Regex library is tested with the [testdata](https://github.com/PCRE2Project/pcre2/tree/master)
-of PCRE2 library.
+of the PCRE2 library.
 
 * testinput1 is from [PCRE2 library](https://github.com/PCRE2Project/pcre2/blob/master/testdata/testinput1),
 * tests for variable length positive lookbehind are removed from testinput1,
